src/Implementations/LogCache/LogCache.v
@@ -1,0 +1,1 @@
+Require Export LogCache.Definitions LogCache.Specs.
